src/LocalsDestsComp.v
@@ -1,0 +1,540 @@
+Require Import Common Monads.
+Require Import Metadata.
+Require String.
+Require StackFlatter2 LocalsDests.
+Require Import ListLemmas.
+Require Import HigherValue.
+
+Require Import Psatz.
+
+Module A := StackFlatter2.
+Module B := LocalsDests.
+
+Add Printing Constructor A.frame.
+Add Printing Constructor B.frame.
+
+
+Section compile.
+Open Scope state_monad.
+
+Definition fresh : state nat nat := fun s => (s, S s).
+
+Notation pure := ret_state.
+
+Definition compile : A.insn -> state nat B.insn :=
+    let fix go e :=
+        let fix go_list (es : list A.insn) : state nat (list B.insn) :=
+            match es with
+            | [] => ret_state []
+            | e :: es => @cons _ <$> go e <*> go_list es
+            end in
+        let fix go_list_list (es : list (list A.insn)) : state nat (list (list B.insn)) :=
+            match es with
+            | [] => ret_state []
+            | e :: es => @cons _ <$> go_list e <*> go_list_list es
+            end in
+        match e with
+        | A.Arg => B.Arg <$> fresh
+        | A.Self => B.Self <$> fresh
+        | A.Deref off => B.Deref <$> fresh <*> pure off
+        | A.Call => B.Call <$> fresh
+        | A.MkConstr tag nargs => B.MkConstr <$> fresh <*> pure tag <*> pure nargs
+        | A.Switch cases => B.Switch <$> fresh <*> go_list_list cases
+        | A.MkClose fname nfree => B.MkClose <$> fresh <*> pure fname <*> pure nfree
+        end in go.
+
+Definition compile_list :=
+    let go := compile in
+    let fix go_list es :=
+        match es with
+        | [] => ret_state []
+        | e :: es => @cons _ <$> go e <*> go_list es
+        end in go_list.
+
+Definition compile_list_list :=
+    let go_list := compile_list in
+    let fix go_list_list es :=
+        match es with
+        | [] => ret_state []
+        | e :: es => @cons _ <$> go_list e <*> go_list_list es
+        end in go_list_list.
+
+Ltac refold_compile :=
+    fold compile_list in *;
+    fold compile_list_list in *.
+
+End compile.
+
+
+
+Inductive I_insn : A.insn -> B.insn -> Prop :=
+| IArg : forall dst,
+        I_insn A.Arg (B.Arg dst)
+| ISelf : forall dst,
+        I_insn A.Self (B.Self dst)
+| IDeref : forall dst off,
+        I_insn (A.Deref off) (B.Deref dst off)
+| ICall : forall dst,
+        I_insn A.Call (B.Call dst)
+| IMkConstr : forall dst tag nargs,
+        I_insn (A.MkConstr tag nargs) (B.MkConstr dst tag nargs)
+| ISwitch : forall dst acases bcases,
+        Forall2 (Forall2 I_insn) acases bcases ->
+        I_insn (A.Switch acases) (B.Switch dst bcases)
+| IMkClose : forall dst fname nfree,
+        I_insn (A.MkClose fname nfree) (B.MkClose dst fname nfree)
+.
+
+Inductive I_frame : A.frame -> B.frame -> Prop :=
+| IFrame : forall arg self astk bstk blocals,
+        Forall2 (fun av bl => lookup blocals bl = Some av) astk bstk ->
+        I_frame (A.Frame arg self astk) (B.Frame arg self bstk blocals).
+Hint Constructors I_frame.
+
+Inductive I_keys : list nat -> list nat -> Prop :=
+| IKeys : forall now later,
+        distinct now ->
+        distinct later ->
+        disjoint now later ->
+        I_keys now later.
+
+Fixpoint collect_keys k :=
+    match k with
+    | B.Kswitch code dst _ k' => dst :: B.dests_list code ++ collect_keys k'
+    | _ => []
+    end.
+
+Inductive I_cont : A.cont -> list (nat * value) -> B.cont -> Prop :=
+| IkRet : forall acode af ak locals bcode bdst bf bk,
+        Forall2 I_insn acode bcode ->
+        I_frame af bf ->
+        I_cont ak (B.locals bf) bk ->
+        I_keys (keys (B.locals bf)) (bdst :: B.dests_list bcode ++ collect_keys bk) ->
+        I_cont (A.Kret acode af ak) locals (B.Kret bcode bdst bf bk)
+| IkSwitch : forall acode astk ak locals bcode bdst bstk bk,
+        Forall2 I_insn acode bcode ->
+        Forall2 (fun av bl => lookup locals bl = Some av) astk bstk ->
+        I_cont ak locals bk ->
+        I_cont (A.Kswitch acode astk ak) locals (B.Kswitch bcode bdst bstk bk)
+| IkStop : forall locals, I_cont A.Kstop locals B.Kstop.
+
+Inductive I : A.state -> B.state -> Prop :=
+| IRun : forall acode af ak  bcode bf bk,
+        Forall2 I_insn acode bcode ->
+        I_frame af bf ->
+        I_cont ak (B.locals bf) bk ->
+        I_keys (keys (B.locals bf)) (B.dests_list bcode ++ collect_keys bk) ->
+        I (A.Run acode af ak)
+          (B.Run bcode bf bk)
+
+| IStop : forall v,
+        I (A.Stop v) (B.Stop v).
+
+
+
+Theorem compile_I_expr : forall a b s s',
+    compile a s = (b, s') ->
+    I_insn a b.
+induction a using A.insn_rect_mut with
+    (Pl := fun a => forall b s s',
+        compile_list a s = (b, s') ->
+        Forall2 I_insn a b)
+    (Pll := fun a => forall b s s',
+        compile_list_list a s = (b, s') ->
+        Forall2 (Forall2 I_insn) a b);
+intros0 Hcomp; simpl in Hcomp; break_bind_state;
+try solve [econstructor; eauto].
+Qed.
+
+
+
+Ltac i_ctor := intros; econstructor; simpl; eauto.
+Ltac i_lem H := intros; eapply H; simpl; eauto.
+
+Ltac stk_simpl := compute [
+    A.pop A.push A.pop_push  A.arg A.self A.stack
+    B.pop B.push B.pop_push  B.arg B.self B.stack B.locals
+    ] in *.
+
+Lemma lookup_some_same : forall A xs k (x : A) k' x',
+    lookup xs k = Some x ->
+    ~ In k' (keys xs) ->
+    lookup ((k', x') :: xs) k = Some x.
+intros0 Hlook Hin. simpl.
+break_if.
+- eapply lookup_some_in_keys in Hlook. subst k'. exfalso. eauto.
+- eauto.
+Qed.
+
+Lemma push_I_frame : forall af bf l v,
+    ~ In l (keys (B.locals bf)) ->
+    I_frame af bf ->
+    I_frame (A.push af v) (B.push bf l v).
+intros0 Hin II. destruct af, bf. stk_simpl.
+invc II. constructor.
+constructor.
+- simpl. break_if; congruence.
+- list_magic_on (stack, (stack0, tt)).
+  eapply lookup_some_same; eauto.
+Qed.
+Hint Resolve push_I_frame.
+
+Lemma pop_I_frame : forall af bf n,
+    I_frame af bf ->
+    I_frame (A.pop af n) (B.pop bf n).
+intros0 II. destruct af, bf. stk_simpl.
+invc II. constructor.
+eauto using Forall2_skipn.
+Qed.
+Hint Resolve pop_I_frame.
+
+Lemma pop_push_I_frame : forall af bf n l v,
+    ~ In l (keys (B.locals bf)) ->
+    I_frame af bf ->
+    I_frame (A.pop_push af n v) (B.pop_push bf n l v).
+intros0 Hin II.
+eapply push_I_frame, pop_I_frame; eauto.
+Qed.
+Hint Resolve pop_push_I_frame.
+
+Lemma disjoint_cons_l_not_in_r : forall A (xs ys : list A) x,
+    disjoint (x :: xs) ys ->
+    ~ In x ys.
+intros0 Hxy. invc Hxy. on >Forall, invc. eauto.
+Qed.
+Hint Resolve disjoint_cons_l_not_in_r.
+
+Lemma disjoint_cons_r_not_in_l : forall A (xs ys : list A) y,
+    disjoint xs (y :: ys) ->
+    ~ In y xs.
+intros0 Hxy. eapply disjoint_sym in Hxy. 
+eauto using disjoint_cons_l_not_in_r.
+Qed.
+Hint Resolve disjoint_cons_r_not_in_l.
+
+Lemma I_keys_move : forall xs y ys,
+    I_keys xs (y :: ys) ->
+    I_keys (y :: xs) ys.
+intros0 II. invc II. constructor.
+- constructor; eauto.
+- on (distinct (_ :: _)), invc. auto.
+- on (distinct (_ :: _)), invc. eapply cons_disjoint_l; eauto.
+Qed.
+Hint Resolve I_keys_move.
+
+Lemma I_keys_sym : forall xs ys,
+    I_keys xs ys ->
+    I_keys ys xs.
+intros0 II. invc II. constructor; eauto. eauto using disjoint_sym.
+Qed.
+
+Lemma I_keys_move' : forall xs x ys,
+    I_keys (x :: xs) ys ->
+    I_keys xs (x :: ys).
+intros0 II. eauto using I_keys_sym, I_keys_move.
+Qed.
+Hint Resolve I_keys_move'.
+
+Lemma I_keys_r_not_in_l : forall xs y ys,
+    I_keys xs (y :: ys) ->
+    ~ In y xs.
+inversion 1. eauto using disjoint_cons_r_not_in_l.
+Qed.
+
+Lemma I_keys_r_not_in_r : forall xs y ys,
+    I_keys xs (y :: ys) ->
+    ~ In y ys.
+inversion 1. on (distinct (_ :: _)), invc. auto.
+Qed.
+
+Lemma I_keys_cons_r_inv : forall xs y ys
+        (P : _ -> _ -> _ -> Prop),
+    (I_keys xs ys ->
+        ~ In y xs ->
+        ~ In y ys ->
+        P xs y ys) ->
+    I_keys xs (y :: ys) -> P xs y ys.
+intros0 HP II.
+eapply HP.
+- invc II. on (distinct (_ :: _)), invc. constructor; eauto.
+- eauto using I_keys_r_not_in_l.
+- eauto using I_keys_r_not_in_r.
+Qed.
+
+Lemma cons_I_keys_l : forall x xs ys,
+    I_keys xs ys ->
+    ~ In x xs ->
+    ~ In x ys ->
+    I_keys (x :: xs) ys.
+intros0 II Hinl Hinr.
+invc II. constructor; eauto.
+constructor; eauto.
+Qed.
+Hint Resolve cons_I_keys_l.
+
+Lemma cons_I_keys_r : forall y xs ys,
+    I_keys xs ys ->
+    ~ In y xs ->
+    ~ In y ys ->
+    I_keys xs (y :: ys).
+intros0 II Hinl Hinr.
+invc II. constructor; eauto.
+constructor; eauto.
+Qed.
+Hint Resolve cons_I_keys_r.
+
+Lemma cons_I_cont : forall ak locals bk  k v,
+    ~ In k (keys locals) ->
+    I_cont ak locals bk ->
+    I_cont ak ((k, v) :: locals) bk.
+first_induction ak; intros0 Hin II; invc II.
+- constructor; eauto.
+- constructor; eauto. list_magic_on (stk, (bstk, tt)).
+  eapply lookup_some_same; eauto.
+- constructor.
+Qed.
+Hint Resolve cons_I_cont.
+
+Lemma I_frame_stack_local : forall af bf idx v,
+    nth_error (A.stack af) idx = Some v ->
+    I_frame af bf ->
+    B.stack_local bf idx = Some v.
+intros0 Hnth II. invc II. unfold B.stack_local. simpl in *.
+fwd eapply Forall2_nth_error_ex; eauto. break_exists. break_and.
+find_rewrite.
+unfold B.local. simpl. auto.
+Qed.
+
+Lemma A_top_nth_error : forall af v,
+    A.top af = v ->
+    length (A.stack af) >= 1 ->
+    nth_error (A.stack af) 0 = Some v.
+intros0 Htop Hlen.
+destruct af. destruct stack.
+  { simpl in *. lia. }
+unfold A.top in Htop. simpl in *. congruence.
+Qed.
+
+Lemma Forall2_rev : forall A B P (xs : list A) (ys : list B),
+    Forall2 P xs ys ->
+    Forall2 P (rev xs) (rev ys).
+induction xs; intros0 Hfa; invc Hfa.
+- simpl. constructor.
+- change (a :: xs) with ([a] ++ xs).
+  change (y :: l') with ([y] ++ l').
+  do 2 rewrite rev_app_distr.
+  eapply Forall2_app; eauto.
+  simpl. eauto.
+Qed.
+
+
+Lemma B_nth_error_dests_list_app : forall iss n is,
+    nth_error iss n = Some is ->
+    exists before after,
+        B.dests_list_list iss = before ++ B.dests_list is ++ after.
+induction iss; intros0 Hnth.
+  { destruct n; discriminate. }
+destruct n; simpl in *.
+- inject_some. exists []. eexists. reflexivity.
+- specialize (IHiss ?? ?? **). break_exists.
+  find_rewrite. rewrite app_assoc. eauto.
+Qed.
+
+Lemma app_distinct_flip' : forall A (xs ys : list A),
+    distinct (xs ++ ys) ->
+    distinct (ys ++ xs).
+intros0 Hxy. invc_using distinct_app_inv Hxy.
+eapply app_distinct; eauto using disjoint_sym.
+Qed.
+
+Lemma app_distinct_flip : forall A (xs ys : list A),
+    distinct (xs ++ ys) <->
+    distinct (ys ++ xs).
+firstorder eauto using app_distinct_flip'.
+Qed.
+
+Lemma app_I_keys_flip_r' : forall xs ys1 ys2,
+    I_keys xs (ys1 ++ ys2) ->
+    I_keys xs (ys2 ++ ys1).
+intros0 II. invc II. constructor; eauto.
+- rewrite app_distinct_flip. auto.
+- on >@disjoint, invc. constructor. list_magic_on (xs, tt).
+  rewrite in_app_iff in *. firstorder.
+Qed.
+
+Lemma app_I_keys_flip_r : forall xs ys1 ys2,
+    I_keys xs (ys1 ++ ys2) <->
+    I_keys xs (ys2 ++ ys1).
+firstorder eauto using app_I_keys_flip_r'.
+Qed.
+
+Lemma cons_app : forall A (x : A) xs,
+    x :: xs = [x] ++ xs.
+intros. reflexivity.
+Qed.
+
+Lemma app_distinct_permut' : forall A (xs ys zs : list A),
+    distinct (xs ++ ys ++ zs) ->
+    distinct (ys ++ xs ++ zs).
+intros0 Hxyz.
+rewrite app_assoc in *.  invc_using distinct_app_inv Hxyz.
+eapply app_distinct; eauto.
+- eauto using app_distinct_flip'.
+- on >@disjoint, invc. constructor.
+  on _, invc_using Forall_app_inv. eauto using Forall_app.
+Qed.
+
+Lemma app_distinct_permut : forall A (xs ys zs : list A),
+    distinct (xs ++ ys ++ zs) <->
+    distinct (ys ++ xs ++ zs).
+firstorder eauto using app_distinct_permut'.
+Qed.
+
+Lemma app_I_keys_permut_r' : forall xs ys1 ys2 ys3,
+    I_keys xs (ys1 ++ ys2 ++ ys3) ->
+    I_keys xs (ys2 ++ ys1 ++ ys3).
+intros0 II. invc II. constructor; eauto.
+- rewrite app_distinct_permut. auto.
+- on >@disjoint, invc. constructor. list_magic_on (xs, tt).
+  do 2 rewrite in_app_iff in *. firstorder.
+Qed.
+
+Lemma app_I_keys_permut_r : forall xs ys1 ys2 ys3,
+    I_keys xs (ys1 ++ ys2 ++ ys3) <->
+    I_keys xs (ys2 ++ ys1 ++ ys3).
+firstorder eauto using app_I_keys_permut_r'.
+Qed.
+
+Lemma overly_specific_I_keys_lemma : forall xs ys1 ys2 ys3 ys4 ys5 y,
+    I_keys xs (((ys1 ++ ys2 ++ ys3) ++ ys4) ++ ys5) ->
+    ~ In y xs ->
+    ~ In y (((ys1 ++ ys2 ++ ys3) ++ ys4) ++ ys5) ->
+    I_keys xs (ys2 ++ y :: ys4 ++ ys5).
+intros0 Hkeys Hinl Hinr.
+rewrite cons_app.
+rewrite app_I_keys_permut_r.
+
+replace (((ys1 ++ ys2 ++ ys3) ++ ys4) ++ ys5)
+   with (ys1 ++ ys2 ++ ys3 ++ ys4 ++ ys5) in Hkeys
+   by (repeat rewrite app_assoc; reflexivity).
+rewrite app_I_keys_flip_r in Hkeys.
+replace ((ys2 ++ ys3 ++ ys4 ++ ys5) ++ ys1)
+   with (ys2 ++ ys3 ++ ys4 ++ ys5 ++ ys1) in Hkeys
+   by (repeat rewrite app_assoc; reflexivity).
+rewrite app_I_keys_permut_r in Hkeys.
+replace (ys3 ++ ys2 ++ ys4 ++ ys5 ++ ys1)
+   with ((ys3 ++ ys2 ++ ys4 ++ ys5) ++ ys1) in Hkeys
+   by (repeat rewrite app_assoc; reflexivity).
+rewrite app_I_keys_flip_r in Hkeys.
+replace (ys1 ++ ys3 ++ ys2 ++ ys4 ++ ys5)
+   with ((ys1 ++ ys3) ++ ys2 ++ ys4 ++ ys5) in Hkeys
+   by (repeat rewrite app_assoc; reflexivity).
+
+simpl. eapply cons_I_keys_r; eauto.
+- invc Hkeys. constructor; eauto.
+  + on _, invc_using distinct_app_inv. auto.
+  + on >@disjoint, invc. constructor. list_magic_on (xs, tt).
+    repeat rewrite in_app_iff in *. firstorder.
+- repeat rewrite in_app_iff in *. firstorder.
+Qed.
+
+
+Theorem I_sim : forall AE BE a a' b,
+    Forall2 (Forall2 I_insn) AE BE ->
+    Forall (fun is => distinct (B.dests_list is)) BE ->
+    I a b ->
+    A.sstep AE a a' ->
+    exists b',
+        B.sstep BE b b' /\
+        I a' b'.
+
+destruct a as [ae al ak | ae];
+intros0 Henv Bdt II Astep; [ | solve [invc Astep] ].
+
+inv Astep; inv II;
+try on (Forall2 I_insn _ _), invc;
+try on (I_insn _ _), invc;
+(*
+try on (Forall2 _ [] _), invc;
+*)
+try on >I_frame, inv;
+try on _, invc_using I_keys_cons_r_inv;
+simpl in *; B.refold_dests; try subst.
+
+
+- (* Arg *)
+  eexists. split. eapply B.SArg; stk_simpl. simpl.
+  i_ctor.
+
+- (* Self *)
+  eexists. split. eapply B.SSelf; stk_simpl. simpl.
+  i_ctor.
+
+- (* DerefinateConstr *)
+  eexists. split. eapply B.SDerefinateConstr; simpl; eauto.
+    { eapply I_frame_stack_local; eauto. eapply A_top_nth_error; eauto. }
+  i_ctor.
+
+- (* DerefinateClose *)
+  eexists. split. eapply B.SDerefinateClose; simpl; eauto.
+    { eapply I_frame_stack_local; eauto. eapply A_top_nth_error; eauto. }
+  i_ctor.
+
+- (* MkConstr *)
+  eexists. split. eapply B.SConstrDone; simpl; eauto.
+    { erewrite <- Forall2_length; eauto. }
+    { unfold B.local. simpl. eapply Forall2_rev, Forall2_firstn.
+      instantiate (1 := astk). list_magic_on (astk, (bstk, tt)). }
+  i_ctor.
+
+- (* MkClose *)
+  eexists. split. eapply B.SCloseDone; simpl; eauto.
+    { erewrite <- Forall2_length; eauto. }
+    { unfold B.local. simpl. eapply Forall2_rev, Forall2_firstn.
+      instantiate (1 := astk). list_magic_on (astk, (bstk, tt)). }
+  i_ctor.
+
+- (* MakeCall *)
+  fwd eapply Forall2_nth_error_ex with (xs := AE) as HH; eauto.  destruct HH as (bbody & ? & ?).
+  destruct astk as [| aarg [| aself astk ] ]; try discriminate. inject_some.
+
+  eexists. split. eapply B.SMakeCall; simpl; eauto.
+    { eapply I_frame_stack_local; eauto. simpl. reflexivity. }
+    { eapply I_frame_stack_local; eauto. simpl. reflexivity. }
+  i_ctor. i_ctor. i_ctor. i_ctor.
+  rewrite app_nil_r. pattern bbody. eapply Forall_nth_error; eauto.
+
+- (* Switchinate *)
+  fwd eapply Forall2_nth_error_ex with (xs := cases) as HH; eauto.  destruct HH as (bcase & ? & ?).
+
+  eexists. split. eapply B.SSwitchinate; eauto using eq_refl.
+  i_ctor. i_ctor.
+  fwd eapply B_nth_error_dests_list_app as HH; eauto.
+    destruct HH as (before & after & Heq). rewrite Heq in *.
+  eapply overly_specific_I_keys_lemma; eauto.
+
+- (* ContRet *)
+  on >I_cont, inv.
+  fwd eapply I_keys_r_not_in_l; eauto.
+
+  eexists. split. eapply B.SContRet; eauto using eq_refl.
+    { eapply I_frame_stack_local; eauto. eapply A_top_nth_error; eauto. }
+  i_ctor.
+
+- (* ContSwitch *)
+  on (Forall2 _ (_ :: _) _), invc. rename y into bv. rename l' into bstk.
+  on >I_cont, inv.
+  fwd eapply I_keys_r_not_in_l; eauto.
+  assert (bstk0 = bstk) by admit. (* need to fix I_cont *) subst bstk0.
+
+  eexists. split. eapply B.SContSwitch; eauto using eq_refl.
+  i_ctor.
+  change (A.Frame _ _ _) with (A.pop_push (A.Frame arg self (v :: stk)) 1 v).
+  eauto using pop_push_I_frame.
+
+- (* ContStop *)
+  on >I_cont, invc.
+  eexists. split. eapply B.SContStop; eauto using eq_refl.
+    { eapply I_frame_stack_local; eauto. eapply A_top_nth_error; eauto. }
+  i_ctor.
+Admitted.
